Core/Beacon.v
@@ -1,0 +1,56 @@
+From mathcomp
+Require Import all_ssreflect.
+From fcsl
+Require Import pred prelude ordtype pcm finmap unionmap heap.
+From CasperToychain
+Require Import CasperOneMessage ValidatorQuorum ValidatorDepositQuorum Blockforest ValidatorBlockforest.
+Set Implicit Arguments.
+Unset Strict Implicit.
+Unset Printing Implicit Defensive.
+
+Record NodeState := 
+ Node {
+   blocks : Blockforest;
+ }.
+  
+Definition NodeInit : NodeState :=
+  Node (#GenesisBlock \\-> GenesisBlock).
+
+Inductive Input :=
+| BlockT of block.
+
+Definition procInp (st : NodeState) (inp : Input) :=
+ let: Node bf := st in
+ match inp with
+ | BlockT b => Node (#b \\-> b \+ bf)
+ end.
+
+Definition Coh (ns : NodeState) :=
+  [/\ valid (blocks ns),     
+     validH (blocks ns) &
+     has_init_block (blocks ns)
+  ].
+
+Inductive system_step (ns ns' : NodeState) : Prop :=
+| Idle of Coh ns /\ ns = ns'
+
+| Intern (inp : Input) of
+   Coh ns & ns' = procInp ns inp.
+
+Definition vote_msg_bf (bf : Blockforest) (v : Validator) (h : Hash) (view : nat) (view_src: nat) : bool :=
+  if find h bf is Some b then
+    [&& block_view b == view & (@mkAR [ordType of Hash] view_src v) \in attestations b]
+  else
+    false.
+
+Definition NodeState_State (ns : NodeState) : State Validator Hash :=
+ mkSt (vote_msg_bf (blocks ns)).
+
+Lemma accountable_safety_NodeState_deposit :
+  forall (deposit : Validator -> nat) (ns : NodeState),
+    finalization_fork (deposit_top_validators deposit) (hash_parent_bf (blocks ns)) (# GenesisBlock) (NodeState_State ns) ->
+    misbehaving_slashed (deposit_bot_validators deposit) (NodeState_State ns).
+Proof.
+move => deposit ns.
+exact: accountable_safety_bf_deposit.
+Qed.
